src/Parsers/DependentlyTypedMinimalOfParseFactored.v
@@ -1,0 +1,406 @@
+(** * Definition of a [comp]-based non-computational CFG parser *)
+Require Import Coq.Lists.List Coq.Program.Program Coq.Program.Wf Coq.Arith.Wf_nat Coq.Arith.Compare_dec Coq.Classes.RelationClasses Coq.Strings.String.
+Require Import Parsers.ContextFreeGrammar Parsers.Specification Parsers.DependentlyTyped Parsers.MinimalParse.
+Require Import Parsers.DependentlyTypedMinimal Parsers.DependentlyTypedOption Parsers.DependentlyTypedSum.
+Require Import Parsers.WellFoundedParse Parsers.ContextFreeGrammarProperties.
+Require Import Common Common.ilist Common.Wf Common.Le.
+
+Set Implicit Arguments.
+
+Local Open Scope string_like_scope.
+
+Local Coercion is_true : bool >-> Sortclass.
+
+Section recursive_descent_parser.
+  Context (CharType : Type)
+          (String : string_like CharType)
+          (G : grammar CharType).
+  Context {predata : parser_computational_predataT}.
+  Local Instance types_data : @parser_computational_types_dataT _ String
+    := {| predata := predata;
+          split_stateT str0 valid g str := True |}.
+  Context {methods' : @parser_computational_dataT' _ String types_data}
+          {strdata : @parser_computational_strdataT _ String G {| methods' := methods' |}}.
+
+  Local Instance orig_methods : @parser_computational_dataT _ String
+    := { methods' := methods' }.
+
+  Context (remove_nonterminal_name_1
+           : forall ls ps ps',
+               is_valid_nonterminal_name (remove_nonterminal_name ls ps) ps' = true
+               -> is_valid_nonterminal_name ls ps' = true)
+          (remove_nonterminal_name_2
+           : forall ls ps ps',
+               is_valid_nonterminal_name (remove_nonterminal_name ls ps) ps' = false
+               <-> is_valid_nonterminal_name ls ps' = false \/ ps = ps').
+
+  Definition P (str0 : String) valid : String -> string -> Prop
+    := fun str p =>
+         sub_names_listT is_valid_nonterminal_name valid initial_nonterminal_names_data
+         /\ is_valid_nonterminal_name
+              (if lt_dec (Length str) (Length str0)
+               then initial_nonterminal_names_data
+               else valid)
+              p = true.
+
+  Lemma P_remove_impl {str0 valid str name name'}
+        (H0 : name <> name')
+        (H : P str0 valid str name')
+  : P str0 (remove_nonterminal_name valid name) str name'.
+  Proof.
+    destruct_head_hnf and.
+    repeat split; try assumption.
+    { apply sub_names_listT_remove_2; assumption. }
+    { destruct lt_dec; try assumption.
+      match goal with
+        | [ |- ?b = true ] => case_eq b; try reflexivity
+      end.
+      intro H'; exfalso.
+      apply remove_nonterminal_name_2 in H'.
+      destruct H'; congruence. }
+  Qed.
+
+  Definition p_parse_item str0 valid s it
+    := { p' : parse_of_item String G s it & Forall_parse_of_item (P str0 valid) p' }.
+  Definition p_parse_production str0 valid s p
+    := { p' : parse_of_production String G s p & Forall_parse_of_production (P str0 valid) p' }.
+  Definition p_parse str0 valid s prods
+    := { p' : parse_of String G s prods & Forall_parse_of (P str0 valid) p' }.
+  Definition p_parse_nonterminal_name str0 valid s nonterminal_name
+    := { p' : parse_of_item String G  s (NonTerminal _ nonterminal_name) & Forall_parse_of_item (P str0 valid) p' }.
+
+  Definition split_parse_of_production {str0 valid str it its}
+             (p : p_parse_production str0 valid str (it::its))
+  : { s1s2 : String * String & (fst s1s2 ++ snd s1s2 =s str)
+                               * p_parse_item str0 valid (fst s1s2) it
+                               * p_parse_production str0 valid (snd s1s2) its }%type.
+  Proof.
+    destruct p as [p H]; revert p H.
+    pattern (it :: its).
+    match goal with
+      | [ |- ?P ?ls ]
+        => set (prods := ls);
+          change it with (hd it prods);
+          change its with (tl prods);
+          assert (H' : ls = prods) by reflexivity;
+          clearbody prods;
+          simpl
+    end.
+    intro p.
+    destruct p.
+    { exfalso; clear -H'; abstract inversion H'. }
+    { intro H''.
+      eexists (_, _); simpl.
+      repeat split; try match goal with H : _ |- _ => exists H end.
+      { apply bool_eq_correct; reflexivity. }
+      { exact (fst H''). }
+      { exact (snd H''). } }
+  Defined.
+
+  Lemma split_parse_of_production_le1 {str0 valid str it its p}
+  : fst (projT1 (@split_parse_of_production str0 valid str it its p)) ≤s str.
+  Proof.
+    etransitivity; [ eapply str_le1_append | right; apply bool_eq_correct ].
+    exact (fst (fst (projT2 (split_parse_of_production p)))).
+  Qed.
+
+  Lemma split_parse_of_production_le2 {str0 valid str it its p}
+  : snd (projT1 (@split_parse_of_production str0 valid str it its p)) ≤s str.
+  Proof.
+    etransitivity; [ eapply str_le2_append | right; apply bool_eq_correct ].
+    exact (fst (fst (projT2 (split_parse_of_production p)))).
+  Qed.
+
+  Local Instance top_types_data : @parser_computational_types_dataT _ String
+    := { split_stateT str0 valid g s
+         := match g return Type with
+              | include_item it => p_parse_item str0 valid s it
+              | include_production p => p_parse_production str0 valid s p
+              | include_productions prods => p_parse str0 valid s prods
+              | include_nonterminal_name nonterminal_name => p_parse_nonterminal_name str0 valid s nonterminal_name
+            end }.
+
+  Local Instance top_methods' : @parser_computational_dataT' _ String top_types_data
+    := { split_string_for_production str0 valid it its s
+         := let st' := split_parse_of_production (state_val s) in
+            ({| string_val := fst (projT1 st') ; state_val := snd (fst (projT2 st')) |},
+             {| string_val := snd (projT1 st') ; state_val := snd (projT2 st') |})::nil }.
+  Proof.
+    intros; subst_body; simpl in *.
+    abstract (do 2 try constructor; edestruct @split_parse_of_production; simpl; intuition).
+  Defined.
+
+  Definition parse_of__of__parse_of_item_lt' {str0 valid str nonterminal_name}
+             (pf : Length str < Length str0)
+             (p : p_parse_nonterminal_name str0 valid str nonterminal_name)
+  : P str0 valid str nonterminal_name * p_parse str initial_nonterminal_names_data str (Lookup G nonterminal_name).
+  Proof.
+    refine (match projT1 p as p' in parse_of_item _ _ str' it'
+                  return match it' with
+                           | Terminal _ => True
+                           | NonTerminal nonterminal_name' => Length str' < Length str0 -> Forall_parse_of_item (P str0 valid) p' -> P str0 valid str' nonterminal_name' * p_parse str' initial_nonterminal_names_data str' (Lookup G nonterminal_name')
+                         end
+            with
+              | ParseTerminal _ => I
+              | ParseNonTerminal _ _ p' => fun pf' H' => (fst H', existT _ p' (expand_forall_parse_of _ _ (snd H')))
+            end pf (projT2 p)).
+    clear -pf'; unfold P in *; simpl;
+    abstract (intros ??; do 2 edestruct lt_dec; intuition).
+  Defined.
+  Definition parse_of__of__parse_of_item_lt {str0 valid str nonterminal_name} pf p
+    := snd (@parse_of__of__parse_of_item_lt' str0 valid str nonterminal_name pf p).
+
+  Definition deloop_right str0 valid str nonterminal_name
+    := p_parse str0 (remove_nonterminal_name valid nonterminal_name) str (Lookup G nonterminal_name).
+
+  Definition deloop_onceT
+    := forall str0 valid str nonterminal_name prods
+              (p : parse_of String G str prods)
+              (pf : str = str0 :> String)
+              (H : Forall_parse_of (P str0 valid) p),
+         p_parse str0 (remove_nonterminal_name valid nonterminal_name) str prods
+         + deloop_right str0 valid str nonterminal_name.
+
+  Definition deloop_once_productionT
+    := forall str0 valid str nonterminal_name prod
+              (p : parse_of_production String G str prod)
+              (pf : str = str0 :> String)
+              (H : Forall_parse_of_production (P str0 valid) p),
+         p_parse_production str0 (remove_nonterminal_name valid nonterminal_name) str prod
+         + deloop_right str0 valid str nonterminal_name.
+
+  Definition deloop_once_item'
+             (deloop_once : deloop_onceT)
+             {str0 valid str nonterminal_name}
+             {it}
+             (p : parse_of_item String G str it)
+             (pf : str = str0 :> String)
+             (H : Forall_parse_of_item (P str0 valid) p)
+  : p_parse_item str0 (remove_nonterminal_name valid nonterminal_name) str it
+    + deloop_right str0 valid str nonterminal_name.
+  Proof.
+    destruct p as [ | nonterminal_name' str'' p' ].
+    { exact (inl (existT _ (ParseTerminal _ _ _) tt)). }
+    { refine (if string_dec nonterminal_name nonterminal_name'
+              then inr (if @deloop_once _ _ _ nonterminal_name' _ p' pf (snd H)
+                        then _
+                        else _)
+              else match @deloop_once _ _ _ nonterminal_name _ p' pf (snd H) with
+                     | inl p''' => inl (existT _ (ParseNonTerminal _ (projT1 p''')) (P_remove_impl _ (fst H), projT2 p'''))
+                     | inr ret => inr ret
+                   end);
+      clear deloop_once;
+      solve [ assumption
+            | subst; assumption ]. }
+  Defined.
+
+  Definition deloop_once'
+             (deloop_once : deloop_onceT)
+             (deloop_once_production : deloop_once_productionT)
+  : deloop_onceT.
+  Proof.
+    intros str0 valid str nonterminal_name pats p pf H.
+    destruct p as [ str' pat' pats' p' | str' pat' pats' p' ].
+    { refine match deloop_once_production str0 valid str' nonterminal_name _ p' pf H with
+               | inl ret => inl (existT _ (ParseHead pats' (projT1 ret)) (projT2 ret))
+               | inr ret => inr ret
+             end. }
+    { refine match deloop_once str0 valid str' nonterminal_name _ p' pf H with
+               | inl ret => inl (existT _ (ParseTail _ (projT1 ret)) (projT2 ret))
+               | inr ret => inr ret
+             end. }
+  Defined.
+
+  Local Ltac deloop_t :=
+    repeat match goal with
+             | _ => assumption
+             | _ => intro
+             | [ H : ?x = ?y |- _ ] => subst x
+             | [ H : ?x = ?y |- _ ] => subst y
+             | [ H : _ ≤s _ |- _ ] => destruct H
+             | _ => progress simpl in *
+             | [ H : _ |- _ ] => rewrite Length_Empty in H
+             | _ => rewrite Length_Empty
+             | [ H : _ < 0 |- _ ] => destruct (Lt.lt_n_0 _ H)
+             | _ => progress destruct_head and
+             | [ |- _ /\ _ ] => split
+             | [ H : sub_names_listT _ _ _ |- is_valid_nonterminal_name _ _ = true ]
+               => (apply H; eapply sub_names_listT_remove; eassumption)
+             | [ H : ~0 < ?n |- _ ]
+               => (let H' := fresh in
+                   destruct (zerop n) as [ | H' ]; [ clear H | destruct (H H') ])
+             | [ H : Length _ = 0 |- _ ] => apply Empty_Length in H
+             | [ H : ?x <> ?x |- _ ] => destruct (H eq_refl)
+             | [ H : context[Length (_ ++ _)] |- _ ] => rewrite <- Length_correct in H
+             | [ H : ~_ < _ + _ |- _ ]
+               => unique pose proof (proj1 (not_lt_plus H))
+             | [ H : ~_ < _ + _ |- _ ]
+               => unique pose proof (proj2 (not_lt_plus H))
+             | [ H : ?T, H' : ~?T |- _ ] => destruct (H' H)
+             | [ H : ~ ?a < ?a + _ |- _ ] => apply not_lt_add_r in H
+             | [ H : ~ ?a < _ + ?a |- _ ] => apply not_lt_add_l in H
+           end.
+
+  Definition deloop_once_production'
+             (deloop_once : deloop_onceT)
+             (deloop_once_production : deloop_once_productionT)
+  : deloop_once_productionT.
+  Proof.
+    intros str0 valid str nonterminal_name pat p pf H.
+    destruct p as [ | str' pat' strs' pats' p' p'' ].
+    { refine (inl (existT _ (ParseProductionNil _ _) tt)). }
+    { (** We must discriminate based on whether or not [str] has already gotten shorter *)
+      destruct (stringlike_dec str' (Empty _)) as [e|e], (stringlike_dec strs' (Empty _)) as [e'|e'];
+      try (assert (pf0 : str' = str0)
+            by (clear -pf e'; abstract (subst strs'; rewrite ?RightId, ?LeftId in pf; exact pf));
+           pose proof (@deloop_once_item' (deloop_once) str0 valid _ nonterminal_name pat' p' pf0 (fst H)) as deloop_once_item;
+           clear deloop_once);
+      try (assert (pf1 : strs' = str0)
+            by (clear -pf e; abstract (subst str'; rewrite ?RightId, ?LeftId in pf; exact pf));
+           specialize (deloop_once_production str0 valid _ nonterminal_name pats' p'' pf1 (snd H)));
+      try (destruct deloop_once_item as [ret|ret];
+           [ | right; repeat first [ subst str' | subst strs' ]; rewrite ?LeftId, ?RightId; assumption ]);
+      try (destruct deloop_once_production as [ret'|ret'];
+           [ | right; repeat first [ subst str' | subst strs' ]; rewrite ?LeftId, ?RightId; assumption ]);
+      left.
+      { (** empty, empty *)
+        exact (existT _ (ParseProductionCons (projT1 ret) (projT1 ret'))
+                      (projT2 ret, projT2 ret')). }
+      { (** empty, nonempty *)
+        refine (existT _ (ParseProductionCons p' (projT1 ret'))
+                       (expand_forall_parse_of_item _ (fst H), projT2 ret')).
+        unfold P in *; simpl.
+        clear -e e' pf1 remove_nonterminal_name_1 remove_nonterminal_name_2.
+        abstract (intros; edestruct lt_dec; deloop_t). }
+      { (** nonempty, empty *)
+        refine (existT _ (ParseProductionCons (projT1 ret) p'')
+                       (projT2 ret, expand_forall_parse_of_production _ _ (snd H))).
+        unfold P in *; simpl.
+        clear -e e' pf0 remove_nonterminal_name_1 remove_nonterminal_name_2.
+        abstract (intros; edestruct lt_dec; deloop_t). }
+      { (** nonempty, nonempty *)
+        refine (existT _ (ParseProductionCons p' p'')
+                       (expand_forall_parse_of_item _ (fst H),
+                        expand_forall_parse_of_production _ _ (snd H)));
+        unfold P in *; simpl;
+        clear -e e' pf remove_nonterminal_name_1 remove_nonterminal_name_2;
+        abstract (intros; edestruct lt_dec; deloop_t). } }
+  Defined.
+
+  Fixpoint deloop_once {str0 valid str nonterminal_name pats} (p : parse_of String G str pats)
+    := @deloop_once' (@deloop_once) (@deloop_once_production) str0 valid str nonterminal_name pats p
+  with deloop_once_production {str0 valid str nonterminal_name pat} (p : parse_of_production String G str pat)
+       := @deloop_once_production' (@deloop_once) (@deloop_once_production) str0 valid str nonterminal_name pat p.
+  Definition deloop_once_item {str0 valid str nonterminal_name it} (p : parse_of_item String G str it)
+    := @deloop_once_item' (@deloop_once) str0 valid str nonterminal_name it p.
+
+  Definition parse_of__of__parse_of_item_eq' {str0 valid str nonterminal_name}
+             (pf : str = str0 :> String)
+             (p : p_parse_nonterminal_name str0 valid str nonterminal_name)
+  : P str0 valid str nonterminal_name * p_parse str0 (remove_nonterminal_name valid nonterminal_name) str (Lookup G nonterminal_name).
+  Proof.
+    refine (match projT1 p as p' in parse_of_item _ _ str' it'
+                  return match it' with
+                           | Terminal _ => True
+                           | NonTerminal nonterminal_name' => str' = str0 -> Forall_parse_of_item (P str0 valid) p' -> P str0 valid str' nonterminal_name' * p_parse str0 (remove_nonterminal_name valid nonterminal_name') str' (Lookup G nonterminal_name')
+                         end
+            with
+              | ParseTerminal _ => I
+              | ParseNonTerminal nonterminal_name' _ p'
+                => fun pf' H' => (fst H', if @deloop_once str0 valid _ nonterminal_name' _ p' pf' (snd H') then _ else _)
+            end pf (projT2 p));
+    assumption.
+  Defined.
+  Definition parse_of__of__parse_of_item_eq {str0 valid str nonterminal_name} pf p
+    := snd (@parse_of__of__parse_of_item_eq' str0 valid str nonterminal_name pf p).
+
+  Definition top_methods : @parser_computational_dataT _ String
+    := {| DependentlyTyped.methods' := top_methods' |}.
+
+  Local Instance top_prestrdata : @parser_computational_prestrdataT _ String G top_methods option
+    := { prelower_nonterminal_name_state str0 valid nonterminal_name str st := Some st;
+         prelower_string_head str0 valid prod prods str st
+         := match projT1 st as p' in parse_of _ _ str' prods' return Forall_parse_of (P str0 valid) p' -> option (p_parse_production str0 valid str' (hd prod prods')) with
+              | ParseHead _ _ _ p' => fun H => Some (existT _ p' H)
+              | ParseTail _ _ _ _ => fun _ => None
+            end (projT2 st);
+         prelower_string_tail str0 valid prod prods str st
+         := match projT1 st as p' in parse_of _ _ str' prods' return Forall_parse_of (P str0 valid) p' -> option (p_parse str0 valid str' (tl prods')) with
+              | ParseTail _ _ _ p' => fun H => Some (existT _ p' H)
+              | ParseHead _ _ _ _ => fun _ => None
+            end (projT2 st);
+         prelift_lookup_nonterminal_name_state_lt str0 valid nonterminal_name str pf := Some ∘ parse_of__of__parse_of_item_lt pf;
+         prelift_lookup_nonterminal_name_state_eq str0 valid nonterminal_name str pf := Some ∘ parse_of__of__parse_of_item_eq pf }.
+
+  Context (split_list_complete : forall str0 valid it its str pf, @split_list_completeT _ String G _ str0 valid it its str pf (split_string_for_production str0 valid it its str)).
+
+  Local Ltac ddestruct H :=
+    (* work around 4035 *) let H' := fresh in rename H into H'; dependent destruction H'.
+
+  Local Ltac t' :=
+    idtac;
+    match goal with
+      | _ => intro
+      | _ => progress simpl in *
+      | _ => discriminate
+      | _ => congruence
+      | _ => progress destruct_head @StringWithSplitState
+      | _ => progress destruct_head_hnf sigT
+      | _ => progress destruct_head_hnf prod
+      | _ => progress destruct_head_hnf and
+      | [ H : ~?T, H' : ?T |- _ ] => destruct (H H')
+      | [ H : (?x =s ?x) = false |- _ ] => erewrite (proj2 (bool_eq_correct _ _ _)) in H by reflexivity
+      | [ H : parse_of_item _ _ _ (Terminal _) |- _ ] => ddestruct H
+      | [ H : parse_of_item _ _ _ (NonTerminal _ _) |- _ ] => ddestruct H
+      | [ H : parse_of_production _ _ _ [] |- _ ] => ddestruct H
+      | [ H : parse_of _ _ _ (_::_) |- _ ] => ddestruct H
+      | [ H : parse_of _ _ _ nil |- _ ] => ddestruct H
+      | [ H : appcontext[if lt_dec ?a ?b then _ else _] |- _ ] => destruct (lt_dec a b)
+    end.
+
+  Local Ltac t := repeat t'.
+
+  Local Obligation Tactic := t.
+
+  Global Program Instance minimal_of_parse_parser_dependent_types_extra_data'
+  : @parser_dependent_types_extra_dataT _ String G
+    := @sum_extra_data
+         _ String G
+         predata
+         methods'
+         (@minimal_parser_dependent_types_success_data' _ String G _)
+         (@minimal_parser_dependent_types_failure_data' _ String G _)
+         strdata
+         (@minimal_parser_dependent_types_extra_success_data' _ String G _ _)
+         (@minimal_parser_dependent_types_extra_failure_data' _ String G _ _ split_list_complete)
+         _
+         top_methods'
+         top_prestrdata
+         _ _ _ _ _ _ _ _ _.
+
+  Definition minimal_parse_nonterminal_name__of__parse
+             (nonterminal_name : string)
+             (s : String)
+             (p : parse_of_item String G s (NonTerminal _ nonterminal_name))
+             (H : Forall_parse_of_item
+                    (fun _ n => is_valid_nonterminal_name initial_nonterminal_names_data n = true)
+                    p)
+  : minimal_parse_of_name String G initial_nonterminal_names_data is_valid_nonterminal_name remove_nonterminal_name s initial_nonterminal_names_data s nonterminal_name.
+  Proof.
+    pose proof (fun H' => @parse_nonterminal_name _ String G minimal_of_parse_parser_dependent_types_extra_data' nonterminal_name s (Some (existT _ p (expand_forall_parse_of_item H' H)))) as H0.
+    simpl in *.
+    unfold T_nonterminal_name_success, T_nonterminal_name_failure in *.
+    simpl in *.
+    destruct H0; destruct_head False; try assumption; [ clear ].
+    unfold P in *; simpl in *.
+    repeat match goal with
+             | _ => assumption
+             | [ H : _ -> _ |- _ ] => specialize (H (reflexivity _))
+             | [ H : False |- _ ] => destruct H
+             | _ => intro
+             | [ |- _ /\ _ ] => split
+             | [ |- appcontext[if lt_dec ?a ?b then _ else _] ]
+               => destruct (lt_dec a b)
+           end.
+    Defined.
+End recursive_descent_parser.
